backend/RefinementInstances.v
@@ -1,11 +1,10 @@
 Require Import Coq.Relations.Relation_Definitions.
 Require Export Refinement.
-Require Import FunInd.
-Require Import Coqlib Maps Errors Integers Floats Lattice Kildall.
-Require Import AST Linking.
-Require Import Values Memory Globalenvs Events Smallstep.
-Require Import Registers Op RTL RTL_Incomplete.
-Require Import ValueDomain ValueAnalysis NeedDomain NeedOp.
+Require Import Coqlib Maps Errors
+               AST
+               Globalenvs
+               RTL RTL_Incomplete
+               ValueDomain.
 
 (* Destructs conjunctions, disjunctions, etc. *)
 Ltac destruct_ctx := 
@@ -29,15 +28,6 @@ Ltac destruct_ctx :=
   end
   ).
 
-Lemma reflRefinableEq {A} (HRA := mkEqRefinable A) : forall a : A, a ⊑ a.
-Proof. reflexivity. Qed.
-
-Hint Resolve reflRefinableEq : core.
-
-Lemma completeTrue {A} (HRA := mkEqRefinable A) (HCA := mkCompleteTrue A) : forall a : A, is_complete a.
-Proof. compute; eauto. Qed.
-  
-Hint Resolve completeTrue : core.
 
 #[export, refine] Instance refinableRes {A} `{Refinable A} : Refinable (res A) := 
 {
@@ -52,27 +42,28 @@ Proof.
   - unfold Relation_Definitions.transitive; intros [] [] [] ? ?; eauto; try contradiction.
     * eapply is_transitive; eauto.
     * subst; eauto.
-  - intros [] []; eauto; try eapply is_right_reflexive; eauto; try contradiction.
+  - unfold reflexive. intros []; eauto; reflexivity.
 Defined.
 
-#[export, refine] Instance completeRes {A} `{Complete A} : Complete (res A) := 
+#[export]
+Instance completeRes {A} `{Complete A} : Complete (res A) := 
   {
     is_complete := fun r => match r with
     | OK x => is_complete x
     | Error _ => True
     end
   }.
-Proof.
-  intros []; eauto; intros; simpl; eauto; unfold refinement; cbn; try apply is_complete_spec; eauto.
-Defined.
 
-#[export] Instance groundRes {A} `{Ground A} : Ground (res A).
-Proof. constructor; intros [] ? []; simpl; try contradiction; intros.
-      - f_equal. eapply is_complete_minimal; eauto.
-      - unfold refinement in H4; cbn in H4; subst; eauto.
+#[export] 
+Instance groundRes {A} `{Ground A} : Ground (res A).
+Proof. 
+  constructor; intros [] ? []; simpl; try contradiction; intros.
+  - f_equal. eapply is_complete_minimal; eauto.
+  - rewrite H3; reflexivity.
 Defined. 
 
-#[export, refine] Instance refinableOption {A} `{Refinable A} : Refinable (option A) := 
+#[export, refine] 
+Instance refinableOption {A} `{Refinable A} : Refinable (option A) := 
 {
   refinement o1 o2 := match o1, o2 with 
   | Some x1, Some x2 => x1 ⊑ x2
@@ -83,26 +74,26 @@ Defined.
 Proof.
   - unfold Relation_Definitions.transitive; intros [] [] [] ? ?; eauto; try contradiction.
     eapply is_transitive; eauto.
-  - intros [] []; eauto; try eapply is_right_reflexive; eauto; try contradiction.
+  - unfold reflexive; intros []; eauto; reflexivity.
 Defined.
 
-#[export, refine] Instance completeOption {A} `{Complete A} : Complete (option A) := 
+#[export] 
+Instance completeOption {A} `{Complete A} : Complete (option A) := 
   {
     is_complete := fun o => match o with
     | Some x => is_complete x
     | None => True
     end
   }.
-Proof.
-  intros []; eauto; intros; simpl; eauto. unfold refinement; cbn; apply is_complete_spec; eauto.
-Defined.
 
-#[export] Instance groundOption {A} `{Ground A} : Ground (option A).
+#[export] 
+Instance groundOption {A} `{Ground A} : Ground (option A).
 Proof. constructor; intros [] ? []; simpl; try contradiction; intros; eauto.
       f_equal. eapply is_complete_minimal; eauto.
 Defined. 
 
-#[export, refine] Instance refinableList {A} `{Refinable A} : Refinable (list A) := 
+#[export, refine] 
+Instance refinableList {A} `{Refinable A} : Refinable (list A) := 
 {
   refinement l1 l2 := let fix aux l1 l2 :=
    match l1, l2 with
@@ -115,11 +106,12 @@ Proof.
   - unfold Relation_Definitions.transitive. induction x; intros; destruct y; eauto; try contradiction.
     destruct z; eauto; try contradiction. destruct H0; destruct H1; split; try eapply is_transitive; eauto.
     eapply IHx; eauto.
-  - intros l1; induction l1; intros []; eauto; try contradiction; simpl. intros []; split; try eapply is_right_reflexive; eauto. 
-  apply IHl1; eauto.
+  - unfold reflexive; intros l1; induction l1; eauto; try contradiction; simpl. 
+    split; eauto; reflexivity. 
 Defined.
 
-#[export, refine] Instance completeList {A} `{Complete A} : Complete (list A) := 
+#[export] 
+Instance completeList {A} `{Complete A} : Complete (list A) := 
   {
     is_complete l := let fix aux l := 
     match l with 
@@ -127,18 +119,16 @@ Defined.
     | x :: xs => is_complete x /\ aux xs
     end in aux l
   }.
-Proof.
-  intros l; induction l; eauto. simpl; intros []; constructor; try eapply is_complete_spec; eauto.
-  apply IHl; eauto.
-Defined.
 
-#[export] Instance groundList {A} `{Ground A} : Ground (list A).
+#[export] 
+Instance groundList {A} `{Ground A} : Ground (list A).
 Proof. constructor; intros l; induction l; intros [] []; try contradiction; eauto.
   intros []. f_equal. eapply is_complete_minimal; eauto.
   apply IHl; eauto.
 Defined.
   
-#[export, refine] Instance refinableSum {A B} `{Refinable A} `{Refinable B} : Refinable (A + B) := 
+#[export, refine] 
+Instance refinableSum {A B} `{Refinable A} `{Refinable B} : Refinable (A + B) := 
 {
   refinement s1 s2 := match s1, s2 with 
   | inl x1, inl x2 => x1 ⊑ x2
@@ -148,47 +138,47 @@ Defined.
 }.
 Proof.
   - unfold Relation_Definitions.transitive; intros [] [] [] ? ?; eauto; try contradiction; eapply is_transitive; eauto.
-  - intros [] []; eauto; try eapply is_right_reflexive; eauto; try contradiction.
+  - unfold reflexive; intros []; eauto; reflexivity.
 Defined.
 
-#[export, refine] Instance completeSum {A B} `{Complete A} `{Complete B} : Complete (A + B) := 
+#[export] 
+Instance completeSum {A B} `{Complete A} `{Complete B} : Complete (A + B) := 
   {
     is_complete := fun s => match s with
     | inl x => is_complete x
     | inr y => is_complete y
     end
   }.
-Proof.
-  intros []; eauto; intros; simpl; eauto; unfold_refinement; eapply is_complete_spec; eauto.
+
+#[export] 
+Instance groundSum {A B} `{Ground A} `{Ground B} : Ground (A + B).
+Proof. constructor; intros [] ?; intros []; try contradiction; intros; eauto; f_equal; eapply is_complete_minimal; eauto.
 Defined.
 
-#[export] Instance groundSum {A B} `{Ground A} `{Ground B} : Ground (A + B).
-Proof. constructor; intros [] ? []; simpl; try contradiction; intros; eauto; f_equal; eapply is_complete_minimal; eauto.
-Defined.
-
-#[export, refine] Instance refinableProd {A B} `{Refinable A} `{Refinable B} : Refinable (A * B) := 
+#[export, refine] 
+Instance refinableProd {A B} `{Refinable A} `{Refinable B} : Refinable (A * B) := 
 {
   refinement p1 p2 := let (x1, y1) := p1 in let (x2, y2) := p2 in x1 ⊑ x2 /\ y1 ⊑ y2
 }.
 Proof.
   - unfold Relation_Definitions.transitive; intros [] [] [] [] []; split; try eapply is_transitive; eauto.
-  - intros [] [] []; split; try eapply is_right_reflexive; eauto.
+  - unfold reflexive; intros []; split; eauto; reflexivity.
 Defined.
 
-#[export, refine] Instance completeProd {A B} `{Complete A} `{Complete B} : Complete (A * B) := 
+#[export] 
+Instance completeProd {A B} `{Complete A} `{Complete B} : Complete (A * B) := 
   {
     is_complete := fun p => let (x, y) := p in is_complete x /\ is_complete y
   }.
-Proof.
-  intros [] []; constructor; try eapply is_complete_spec; eauto.
-Defined.
 
-#[export] Instance groundProd {A B} `{Ground A} `{Ground B} : Ground (A * B).
+#[export] 
+Instance groundProd {A B} `{Ground A} `{Ground B} : Ground (A * B).
 Proof. constructor; intros [] [] [] []; f_equal; eapply is_complete_minimal; eauto. 
 Defined. 
 
-Arguments monotone {A} {H} {HAC} P {Monotonizable}.
-#[export, refine] Instance monoForall2 {A B C} `{Complete C} (l1 : list A) (l2 : list B) (f : C -> A -> B -> Prop) 
+
+#[export, refine] 
+Instance monoForall2 {C} `{Refinable C} `{Complete C} {A} (l1 : list A) {B} (l2 : list B) (f : C -> A -> B -> Prop) 
   {Hf : forall a b, Monotonizable (fun c => f c a b)} : Monotonizable (fun c => list_forall2 (f c) l1 l2) := 
 {
   monotone := fun c => list_forall2 (fun a b => monotone (fun c => f c a b) c) l1 l2;
@@ -203,62 +193,6 @@ Proof.
   - intros c ?; split; induction 1; econstructor; eauto; eapply (Hf a1 b1).(complete_antitone_is_equivalent); eauto.
 Defined.
   
-(* node and reg are positive *)
-#[export] Instance : Refinable reg := mkEqRefinable reg.
-#[export] Instance : Complete reg := mkCompleteTrue reg. 
-
-#[export] Instance : Refinable operation := mkEqRefinable operation.
-#[export] Instance : Complete operation := mkCompleteTrue operation.
-
-#[export] Instance : Refinable memory_chunk := mkEqRefinable memory_chunk.
-#[export] Instance : Complete memory_chunk := mkCompleteTrue memory_chunk.
-
-#[export] Instance : Refinable addressing := mkEqRefinable addressing. 
-#[export] Instance : Complete addressing := mkCompleteTrue addressing.
-
-(* Signature is actually a record *)
-#[export] Instance : Refinable signature := mkEqRefinable signature.
-#[export] Instance : Complete signature := mkCompleteTrue signature.
-
-(* external_function is an inductive *)
-#[export] Instance : Refinable external_function := mkEqRefinable external_function.
-#[export] Instance : Complete external_function := mkCompleteTrue external_function.
-
-#[export] Instance : Refinable condition := mkEqRefinable condition.
-#[export] Instance : Complete condition := mkCompleteTrue condition.
-
-(* builtin_arg and res are parameterized, so one could have a more general definition *)
-#[export] Instance : Refinable (builtin_arg reg) := mkEqRefinable (builtin_arg reg).
-#[export] Instance : Complete (builtin_arg reg) := mkCompleteTrue (builtin_arg reg).
-
-#[export] Instance : Refinable (builtin_res reg) := mkEqRefinable (builtin_res reg).
-#[export] Instance : Complete (builtin_res reg) := mkCompleteTrue (builtin_res reg).
-
-#[export] Instance : Refinable ablock := mkEqRefinable ablock.
-#[export] Instance : Complete ablock := mkCompleteTrue ablock.
-
-#[export] Instance : Refinable Z := mkEqRefinable Z.
-#[export] Instance : Complete Z := mkCompleteTrue Z . 
-
-#[export] Instance : Refinable init_data := mkEqRefinable init_data.
-#[export] Instance : Complete init_data := mkCompleteTrue init_data.
-
-#[export] Instance : Refinable bool := mkEqRefinable bool.
-#[export] Instance : Complete bool := mkCompleteTrue bool.
-
-#[export] Instance : Refinable ident := mkEqRefinable ident.
-
-#[export] Instance : Refinable unit := mkEqRefinable unit.
-#[export] Instance : Complete unit := mkCompleteTrue unit.
-
-#[export] Instance : Refinable val := mkEqRefinable val.
-#[export] Instance : Complete val := mkCompleteTrue val.
-
-#[export] Instance : Refinable mem := mkEqRefinable mem.
-#[export] Instance : Complete mem := mkCompleteTrue mem.
-
-#[export] Instance : Refinable RTL.instruction := mkEqRefinable RTL.instruction.
-#[export] Instance : Complete RTL.instruction := mkCompleteTrue RTL.instruction.
 
 #[local] Obligation Tactic := idtac.
 
@@ -278,7 +212,8 @@ match i1, i2 with
 | _ , _ => False
 end.
 
-#[export] Program Instance refinableInstruction : Refinable instruction :=
+#[export] 
+Program Instance refinableInstruction : Refinable instruction :=
   {|
     refinement i1 i2 := refinement_instruction i1 i2
   |}.
@@ -288,9 +223,8 @@ end.
     all: destruct_ctx; repeat split; etransitivity; eauto.
   Qed. 
   Next Obligation.
-    intros [] [] H; cbn in *; eauto. 
-    all: try solve [inversion H].
-    all: destruct_ctx; repeat split; eapply is_right_reflexive; eauto.
+    unfold reflexive. intros []; cbn; eauto;
+      try repeat split; reflexivity; eauto.
   Qed. 
   
 Inductive is_complete_instruction : instruction -> Prop :=
@@ -305,17 +239,15 @@ Inductive is_complete_instruction : instruction -> Prop :=
 | is_complete_Ijumptable : forall r n, is_complete r -> is_complete n -> is_complete_instruction (Ijumptable r n)
 | is_complete_Ireturn : forall mr, is_complete mr -> is_complete_instruction (Ireturn mr).
 
-#[export] Program Instance completeInstruction : Complete instruction := 
+#[export] 
+Instance completeInstruction : Complete instruction := 
 { 
   is_complete := is_complete_instruction
 }.
-Next Obligation.
-  intros []; inversion 1; cbn in *; red; cbn. 
-  all: destruct_ctx; repeat split; eapply is_complete_spec; eauto.
-Qed. 
 
 
-#[export, refine ] Instance groundInstruction : Ground instruction := {}. 
+#[export, refine] 
+Instance groundInstruction : Ground instruction := {}. 
 Proof.
   intros []; inversion 1; intros [] Href; red in Href; cbn in *.
   all: try solve [inversion Href].
@@ -323,7 +255,8 @@ Proof.
   all: eapply is_complete_minimal; eauto.
  Qed.  
 
-#[export] Program Instance refinablePTree {A} `{Refinable A} : Refinable (PTree.t A) := 
+#[export] 
+Program Instance refinablePTree {A} `{Refinable A} : Refinable (PTree.t A) := 
 {
   refinement t1 t2 := forall pc, t1 ! pc ⊑ t2 ! pc  
 }.
@@ -331,35 +264,41 @@ Next Obligation.
   red; intros. etransitivity; eauto.
 Qed.    
 Next Obligation.
-  cbn; intros. eapply is_right_reflexive; eauto.
+  unfold reflexive; cbn; intros. reflexivity; eauto.
 Qed.    
 
-#[export] Program Instance completePTree {A} `{Complete A} : Complete (PTree.t A) := 
+#[export] 
+Instance completePTree {A} `{Complete A} : Complete (PTree.t A) := 
 {
   is_complete t := forall pc, is_complete (t ! pc)
 }.
-Next Obligation.
-  cbn; intros; red; cbn. intro. eapply is_complete_spec; eauto.
-Qed.
 
-#[export] Program Instance groundPTree {A} `{Ground A} : Ground (PTree.t A).
+#[export] 
+Program Instance groundPTree {A} `{Ground A} : Ground (PTree.t A).
 Next Obligation.
-  cbn; intros; cbn. eapply PTree.extensionality. intro p; specialize (H4 p).
+  intros ? ? ? ? a Hc a' Hprec. eapply PTree.extensionality. intro p; specialize (Hc p).
   eapply is_complete_minimal; eauto.
 Qed.
 
-#[export] Instance : Refinable romem. apply refinablePTree. Defined.
-#[export] Instance : Complete romem. apply completePTree. Defined.
+#[export] 
+Instance : Refinable romem. apply refinablePTree. Defined.
+#[export] 
+Instance : Complete romem. apply completePTree. Defined.
+
 Lemma romem_complete : forall r : romem, is_complete r. 
 Proof. intros; unfold_complete; intros; unfold_complete; destruct (_ ! _); try unfold_complete; eauto. Qed.
+
+#[export]
+Hint Resolve romem_complete.
+
 Lemma romem_sp : forall r : romem, r ⊑ r. 
 Proof. intros; unfold_refinement; intros; unfold_refinement; destruct (_ ! _); try unfold_refinement; eauto. Qed.
 
+#[export]
+Hint Resolve romem_sp.
 
-#[export] Instance : Refinable RTL.function := mkEqRefinable RTL.function.
-#[export] Instance : Complete RTL.function := mkCompleteTrue RTL.function.
-
-#[export, refine] Instance : Refinable function := 
+#[export, refine] 
+Instance : Refinable function := 
   {
     refinement f1 f2 := 
     (fn_sig f1) ⊑ (fn_sig f2) /\ (fn_params f1) ⊑ (fn_params f2) /\ (fn_stacksize f1) ⊑ (fn_stacksize f2) /\ (fn_code f1) ⊑ (fn_code f2) /\ (fn_entrypoint f1) ⊑ (fn_entrypoint f2)
@@ -368,58 +307,20 @@ Proof.
   - unfold Relation_Definitions.transitive; intros [] [] [] ? ?.
     destruct_ctx.
     repeat split; try eapply is_transitive; eauto.
-  - intros [] [] ?; destruct_ctx. repeat split; try eapply is_right_reflexive; eauto.
+  - unfold reflexive; intros; repeat split; reflexivity; eauto.
 Defined.
 
 
-#[export] Program Instance : Complete function := {
+#[export] 
+Instance : Complete function := {
   is_complete f := 
   is_complete (fn_sig f) /\ is_complete (fn_params f) /\ is_complete (fn_stacksize f) /\ is_complete (fn_code f) /\ is_complete (fn_entrypoint f)
-  (* forall pc, is_complete pc -> is_complete ((fn_code f) ! pc) *)
 }.
-Next Obligation.
-  cbn; intros. destruct_ctx. red; cbn. repeat split; eauto; eapply is_complete_spec; eauto.
-Qed. 
 
-#[export] Instance : Ground function.
+#[export] 
+Instance : Ground function.
 Proof. constructor. intros [] HC [] HR. unfold_complete in HC; unfold_refinement in HR. destruct_ctx. unshelve f_equal; unshelve eapply is_complete_minimal; eauto; try typeclasses eauto.
 Defined.
-
-(*
-
-#[export] Program Instance refinableGlobvar {V} `{Refinable V} : Refinable (globvar V) := 
-{
-  refinement g1 g2 := (gvar_info g1) ⊑ (gvar_info g2) /\ (gvar_init g1) ⊑ (gvar_init g2) /\ (gvar_readonly g1) ⊑ (gvar_readonly g2) /\ (gvar_volatile g1) ⊑ (gvar_volatile g2)
-}.
-Next Obligation. 
-Admit Obligations.
-
-#[export] Program Instance completeGlobvar {V} `{Complete V} : Complete (globvar V) := 
-{
-  is_complete g := is_complete (gvar_info g) /\ is_complete (gvar_init g) /\ is_complete (gvar_readonly g) /\ is_complete (gvar_volatile g)
-}.
-Admit Obligations.
-
-Inductive refinement_globdef {F V} `{Refinable F} `{Refinable V} : globdef F V -> globdef F V -> Prop :=
-| refinement_Gfun : forall f1 f2, f1 ⊑ f2 -> refinement_globdef (Gfun f1) (Gfun f2)
-| refinement_Gvar : forall v1 v2, v1 ⊑ v2 -> refinement_globdef (Gvar v1) (Gvar v2).
-
-#[export] Program Instance refinableGlobdef {F V} `{Refinable F} `{Refinable V} : Refinable (globdef F V) := 
-{
-  refinement := refinement_globdef
-}.
-Admit Obligations.
-
-Inductive is_complete_globdef {F V} `{Complete F} `{Complete V} : globdef F V -> Prop :=
-| is_complete_Gfun : forall f, is_complete f -> is_complete_globdef (Gfun f)
-| is_complete_Gvar : forall v, is_complete v -> is_complete_globdef (Gvar v).
-
-#[export] Program Instance completeGlobdef {F V} `{Complete F} `{Complete V} : Complete (globdef F V) := 
-{
-  is_complete := is_complete_globdef
-}.
-Admit Obligations.
-*)
 
 Definition refinementFunDef {F} `{Refinable F} : relation (AST.fundef F) := fun fd1 fd2 =>
   match fd1, fd2 with
@@ -428,7 +329,8 @@ Definition refinementFunDef {F} `{Refinable F} : relation (AST.fundef F) := fun 
   | _, _ => False
   end.
 
-#[export] Program Instance refinableASTFundef {F} `{Refinable F} : Refinable (AST.fundef F) := 
+#[export]
+Program Instance refinableASTFundef {F} `{Refinable F} : Refinable (AST.fundef F) := 
 {
   refinement := refinementFunDef 
 }.
@@ -436,14 +338,14 @@ Next Obligation.
   red; cbn; intros ? ? [] [] []; cbn; eauto. 
   all: try inversion 1; try inversion 2.
   all: try etransitivity; eauto.
+  reflexivity.
 Qed. 
 Next Obligation.
-  red; cbn; intros ? ? [] []; cbn; eauto. 
-  all: try inversion 1; try inversion 2.
-  eapply is_right_reflexive; eauto.
+  red. intros ? ? []; cbn; eauto; reflexivity. 
 Qed. 
 
-#[export] Program Instance completeASTFundef {F} `{Complete F} : Complete (AST.fundef F) := 
+#[export]
+Instance completeASTFundef {F} `{Complete F} : Complete (AST.fundef F) := 
 {
   is_complete fd := 
     match fd with
@@ -451,25 +353,23 @@ Qed.
     | Internal f => is_complete f
     end
 }.
-Next Obligation.
-  red; cbn; intros ? ? [] []; cbn; eauto. 
-Qed. 
 
-
-#[export] Instance groundASTFundef {F} `{Ground F} : Ground (AST.fundef F).
+#[export] 
+Instance groundASTFundef {F} `{Ground F} : Ground (AST.fundef F).
 Proof. constructor. intros [] ? [] ?; try contradiction;
   try f_equal; eauto; eapply is_complete_minimal; eauto.
 Qed.
 
+#[export] 
+Instance : Refinable fundef. apply refinableASTFundef. Defined.
+#[export] 
+Instance : Complete fundef. apply completeASTFundef. Defined.
+#[export] 
+Instance : Ground fundef. apply groundASTFundef.  Defined. 
 
-#[export] Instance : Refinable fundef. apply refinableASTFundef. Defined.
-#[export] Instance : Complete fundef. apply completeASTFundef. Defined.
-#[export] Instance : Ground fundef. apply groundASTFundef.  Defined. 
 
-#[export] Instance : Refinable RTL.program := mkEqRefinable RTL.program.
-#[export] Instance : Complete RTL.program := mkCompleteTrue RTL.program.
-
-#[export] Program Instance refinableASTProgram : Refinable program := 
+#[export] 
+Program Instance refinableASTProgram : Refinable program := 
 {
   refinement p1 p2 := forall ros rs, find_function (Genv.globalenv p1) ros rs ⊑ find_function (Genv.globalenv p2) ros rs
 }.
@@ -477,22 +377,22 @@ Next Obligation.
   red; cbn; intros. etransitivity; eauto.
 Qed. 
 Next Obligation.
-  cbn; intros. eapply is_right_reflexive; eauto.
+  unfold reflexive; intros; reflexivity.
 Qed. 
 
-#[export] Program Instance completeASTProgram : Complete program := 
+#[export] 
+Instance completeASTProgram : Complete program := 
 {
   is_complete p := (forall ros rs, is_complete (find_function (Genv.globalenv p) ros rs)) /\ forall b, is_complete (Genv.find_funct_ptr (Genv.globalenv p) b)
 }.
-Next Obligation.
-  red; cbn; intros. destruct_ctx. eapply is_complete_spec; eauto.
-Qed. 
 
-#[export] Instance : Refinable program. apply refinableASTProgram. Defined.
-#[export] Instance : Complete program. apply completeASTProgram. Defined.
-(* #[export, refine] Instance : Ground program := {}. *)
+#[export]
+Instance : Refinable program. apply refinableASTProgram. Defined.
+#[export]
+Instance : Complete program. apply completeASTProgram. Defined.
  
-#[export, refine] Instance : Refinable stackframe := 
+#[export, refine] 
+Instance : Refinable stackframe := 
 {
   refinement '(Stackframe r1 f1 v1 n1 rs1) '(Stackframe r2 f2 v2 n2 rs2) := 
   r1 ⊑ r2 /\ f1 ⊑ f2 /\ v1 ⊑ v2 /\ n1 ⊑ n2 /\ rs1 ⊑ rs2
@@ -501,8 +401,7 @@ Proof.
   - unfold Relation_Definitions.transitive; intros [] [] [] ? ?; destruct_ctx.
     unfold_refinement in H7; unfold_refinement in H0; destruct_ctx. 
     repeat split; eapply is_transitive; eauto.
-  - intros [] [] ?; destruct_ctx. unfold_refinement in H2; destruct_ctx.
-    repeat split; try eapply is_right_reflexive; eauto.
+  - unfold reflexive; intros []; repeat split; reflexivity.
 Defined.
 
 Inductive refinement_state : state -> state -> Prop :=
@@ -513,7 +412,8 @@ Inductive refinement_state : state -> state -> Prop :=
 | refinement_Returnstate : forall sfr1 sfr2 v1 v2 m1 m2, 
   sfr1 ⊑ sfr2 -> v1 ⊑ v2 -> m1 ⊑ m2 -> refinement_state (Returnstate sfr1 v1 m1) (Returnstate sfr2 v2 m2).
 
-#[export] Program Instance : Refinable state := 
+#[export] 
+Program Instance : Refinable state := 
 {
   refinement := refinement_state
 }.
@@ -521,5 +421,5 @@ Next Obligation.
   intros ? ? ? []; inversion 1; constructor; etransitivity; eauto.
 Qed. 
 Next Obligation.
-  intros ? ? []; constructor; eapply is_right_reflexive; eauto.
+  unfold reflexive; intros []; constructor; reflexivity.
 Qed.
